PREFIX dcterms: <http://purl.org/dc/terms/>
PREFIX foaf: <http://xmlns.com/foaf/0.1/>
PREFIX owl: <http://www.w3.org/2002/07/owl#>
PREFIX rdfs: <http://www.w3.org/2000/01/rdf-schema#>
PREFIX schema: <https://schema.org/>
PREFIX skos: <http://www.w3.org/2004/02/skos/core#>
PREFIX xsd: <http://www.w3.org/2001/XMLSchema#>

<http://www.neii.gov.au/def/voc/waterprogram/water-market-reports>
    a rdfs:Resource ;
    dcterms:contributor <https://linked.data.gov.au/org/neii> ;
.

<http://www.neii.gov.au/def/voc/waterprogram/water-market-reports/Non-consumptive-use>
    a skos:Concept ;
    dcterms:created "2020-09-07"^^xsd:date ;
    dcterms:creator <https://linked.data.gov.au/org/neii> ;
    skos:definition "Non-consumptive use is when there is no diversion from or diminishment of resource, for example water used to generate hydroelectricity. Held and planned environmental water is a non-consumptive water use."@en ;
    skos:prefLabel "Non-consumptive use"@en ;
    skos:topConceptOf <http://www.neii.gov.au/def/voc/waterprogram/water-market-reports/Water-Market-Reports-glossary> ;
.

<http://www.neii.gov.au/def/voc/waterprogram/water-market-reports/allocation-volume>
    a skos:Concept ;
    dcterms:created "2020-09-07"^^xsd:date ;
    dcterms:creator <https://linked.data.gov.au/org/neii> ;
    skos:definition "The specific volume of water allocated to water access entitlements."@en ;
    skos:prefLabel "allocation volume"@en ;
    skos:topConceptOf <http://www.neii.gov.au/def/voc/waterprogram/water-market-reports/Water-Market-Reports-glossary> ;
.

<http://www.neii.gov.au/def/voc/waterprogram/water-market-reports/available-water>
    a skos:Concept ;
    dcterms:created "2020-09-07"^^xsd:date ;
    dcterms:creator <https://linked.data.gov.au/org/neii> ;
    skos:definition "Water potentially available for consumptive or environmental use."@en ;
    skos:prefLabel "available water"@en ;
    skos:topConceptOf <http://www.neii.gov.au/def/voc/waterprogram/water-market-reports/Water-Market-Reports-glossary> ;
.

<http://www.neii.gov.au/def/voc/waterprogram/water-market-reports/bulk-water>
    a skos:Concept ;
    dcterms:created "2020-09-07"^^xsd:date ;
    dcterms:creator <https://linked.data.gov.au/org/neii> ;
    skos:definition "Water supplied by a water provider to another water provider."@en ;
    skos:prefLabel "bulk water"@en ;
    skos:topConceptOf <http://www.neii.gov.au/def/voc/waterprogram/water-market-reports/Water-Market-Reports-glossary> ;
.

<http://www.neii.gov.au/def/voc/waterprogram/water-market-reports/bulk-water-access-entitlement>
    a skos:Concept ;
    dcterms:created "2020-09-07"^^xsd:date ;
    dcterms:creator <https://linked.data.gov.au/org/neii> ;
    skos:definition "A water access entitlement allowing an infrastructure operator to access, take and hold water for the supply of water to another person."@en ;
    skos:prefLabel "bulk water access entitlement"@en ;
    skos:topConceptOf <http://www.neii.gov.au/def/voc/waterprogram/water-market-reports/Water-Market-Reports-glossary> ;
.

<http://www.neii.gov.au/def/voc/waterprogram/water-market-reports/bundled-right>
    a skos:Concept ;
    dcterms:created "2020-09-07"^^xsd:date ;
    dcterms:creator <https://linked.data.gov.au/org/neii> ;
    skos:definition "The aggregation of individual rights into a single right.  These might include but are not limited to: land property title, water access entitlement, water allocations, water use right, delivery rights, irrigation rights and works approvals."@en ;
    skos:prefLabel "bundled right"@en ;
    skos:topConceptOf <http://www.neii.gov.au/def/voc/waterprogram/water-market-reports/Water-Market-Reports-glossary> ;
.

<http://www.neii.gov.au/def/voc/waterprogram/water-market-reports/carryover>
    a skos:Concept ;
    dcterms:created "2020-09-07"^^xsd:date ;
    dcterms:creator <https://linked.data.gov.au/org/neii> ;
    skos:definition "The option to hold in storage a portion of unused seasonal allocations for use at a later date."@en ;
    skos:prefLabel "carryover"@en ;
    skos:topConceptOf <http://www.neii.gov.au/def/voc/waterprogram/water-market-reports/Water-Market-Reports-glossary> ;
.

<http://www.neii.gov.au/def/voc/waterprogram/water-market-reports/catchment-area>
    a skos:Concept ;
    dcterms:created "2020-09-07"^^xsd:date ;
    dcterms:creator <https://linked.data.gov.au/org/neii> ;
    skos:definition "The extent of land where water from precipitation drains into the water storage."@en ;
    skos:prefLabel "catchment area"@en ;
    skos:topConceptOf <http://www.neii.gov.au/def/voc/waterprogram/water-market-reports/Water-Market-Reports-glossary> ;
.

<http://www.neii.gov.au/def/voc/waterprogram/water-market-reports/consumptive-pool>
    a skos:Concept ;
    dcterms:created "2020-09-07"^^xsd:date ;
    dcterms:creator <https://linked.data.gov.au/org/neii> ;
    skos:definition "The amount of a water resource that can be made available for consumptive use in a particular water resource plan under the rules of the water resource plan for that water resource plan area."@en ;
    skos:prefLabel "consumptive pool"@en ;
    skos:topConceptOf <http://www.neii.gov.au/def/voc/waterprogram/water-market-reports/Water-Market-Reports-glossary> ;
.

<http://www.neii.gov.au/def/voc/waterprogram/water-market-reports/consumptive-use>
    a skos:Concept ;
    dcterms:created "2020-09-07"^^xsd:date ;
    dcterms:creator <https://linked.data.gov.au/org/neii> ;
    skos:definition "Use of water for private benefit consumptive purposes including irrigation, industry, urban and stock and domestic use."@en ;
    skos:prefLabel "consumptive use"@en ;
    skos:topConceptOf <http://www.neii.gov.au/def/voc/waterprogram/water-market-reports/Water-Market-Reports-glossary> ;
.

<http://www.neii.gov.au/def/voc/waterprogram/water-market-reports/external-trade>
    a skos:Concept ;
    dcterms:created "2020-09-07"^^xsd:date ;
    dcterms:creator <https://linked.data.gov.au/org/neii> ;
    skos:definition "A transaction to transfer a water right from one legal entity to another out of a specified area.  The area can be a water system, water management area or a trading zone as defined in respective State and Territory legislation."@en ;
    skos:prefLabel "external trade"@en ;
    skos:topConceptOf <http://www.neii.gov.au/def/voc/waterprogram/water-market-reports/Water-Market-Reports-glossary> ;
.

<http://www.neii.gov.au/def/voc/waterprogram/water-market-reports/gross-water-price>
    a skos:Concept ;
    dcterms:created "2020-09-07"^^xsd:date ;
    dcterms:creator <https://linked.data.gov.au/org/neii> ;
    skos:definition "The transfer price of water as agreed between legal entities inclusive of all applicable transaction costs."@en ;
    skos:prefLabel "gross water price"@en ;
    skos:topConceptOf <http://www.neii.gov.au/def/voc/waterprogram/water-market-reports/Water-Market-Reports-glossary> ;
.

<http://www.neii.gov.au/def/voc/waterprogram/water-market-reports/groundwater>
    a skos:Concept ;
    dcterms:created "2020-09-07"^^xsd:date ;
    dcterms:creator <https://linked.data.gov.au/org/neii> ;
    skos:definition """(a) water occurring naturally below ground level (whether in an aquifer or otherwise) or (b) water occurring at a place below ground that has been pumped, diverted or released to that place for the purpose of being stored there. It does not include water held in underground tanks, pipes or other works. 
Source: Water Act 2007 (https://www.legislation.gov.au/Details/C2018C00505) Part 1 Section 4, at 8 February 2019. For the latest information on Australian Government law please go to Federal Register of Legislation (https://www.legislation.gov.au/)"""@en ;
    skos:prefLabel "groundwater"@en ;
    skos:topConceptOf <http://www.neii.gov.au/def/voc/waterprogram/water-market-reports/Water-Market-Reports-glossary> ;
.

<http://www.neii.gov.au/def/voc/waterprogram/water-market-reports/held-environmental-water>
    a skos:Concept ;
    dcterms:created "2020-09-07"^^xsd:date ;
    dcterms:creator <https://linked.data.gov.au/org/neii> ;
    skos:definition """water available under:
(a) a water access right; or
(b) a water delivery right; or
(c) an irrigation right;
for the purposes of achieving environmental outcomes (including water that is specified in a water access right to be for environmental use).
Source: Water Act 2007 (https://www.legislation.gov.au/Details/C2018C00505) Part 1 Section 4, at 8 February 2019. For the latest information on Australian Government law please go to Federal Register of Legislation (https://www.legislation.gov.au/)"""@en ;
    skos:prefLabel "held environmental water"@en ;
    skos:topConceptOf <http://www.neii.gov.au/def/voc/waterprogram/water-market-reports/Water-Market-Reports-glossary> ;
.

<http://www.neii.gov.au/def/voc/waterprogram/water-market-reports/inflows>
    a skos:Concept ;
    dcterms:created "2020-09-07"^^xsd:date ;
    dcterms:creator <https://linked.data.gov.au/org/neii> ;
    skos:definition "Surface water runoff and deep drainage to groundwater (groundwater recharge) and transfers into the water system (both surface and groundwater) for a defined area."@en ;
    skos:prefLabel "inflows"@en ;
    skos:topConceptOf <http://www.neii.gov.au/def/voc/waterprogram/water-market-reports/Water-Market-Reports-glossary> ;
.

<http://www.neii.gov.au/def/voc/waterprogram/water-market-reports/internal-trade>
    a skos:Concept ;
    dcterms:created "2020-09-07"^^xsd:date ;
    dcterms:creator <https://linked.data.gov.au/org/neii> ;
    skos:definition "A transaction to transfer a water right from one legal entity to another within a specified area.  The area can be a trading zone, irrigation district or a water resource plan area as defined in respective State and Territory legislation."@en ;
    skos:prefLabel "internal trade"@en ;
    skos:topConceptOf <http://www.neii.gov.au/def/voc/waterprogram/water-market-reports/Water-Market-Reports-glossary> ;
.

<http://www.neii.gov.au/def/voc/waterprogram/water-market-reports/interstate-trade>
    a skos:Concept ;
    dcterms:created "2020-09-07"^^xsd:date ;
    dcterms:creator <https://linked.data.gov.au/org/neii> ;
    skos:definition "A transaction to transfer a water right from one legal entity to another in a different State or Territory."@en ;
    skos:prefLabel "interstate trade"@en ;
    skos:topConceptOf <http://www.neii.gov.au/def/voc/waterprogram/water-market-reports/Water-Market-Reports-glossary> ;
.

<http://www.neii.gov.au/def/voc/waterprogram/water-market-reports/intrastate-trade>
    a skos:Concept ;
    dcterms:created "2020-09-07"^^xsd:date ;
    dcterms:creator <https://linked.data.gov.au/org/neii> ;
    skos:definition "A transaction to transfer a water right from one legal entity to another within the same State or Territory."@en ;
    skos:prefLabel "intrastate trade"@en ;
    skos:topConceptOf <http://www.neii.gov.au/def/voc/waterprogram/water-market-reports/Water-Market-Reports-glossary> ;
.

<http://www.neii.gov.au/def/voc/waterprogram/water-market-reports/irrigation-right>
    a skos:Concept ;
    dcterms:created "2020-09-07"^^xsd:date ;
    dcterms:creator <https://linked.data.gov.au/org/neii> ;
    skos:definition """A right that: (a) a person has against an irrigation infrastructure operator to receive water and (b) is not a water access right or a water delivery right.
Source: Water Act 2007 (https://www.legislation.gov.au/Details/C2018C00505) Part 1 Section 4, at 8 February 2019.  For the latest information on Australian Government law please go to Federal Register of Legislation (https://www.legislation.gov.au/)"""@en ;
    skos:prefLabel "irrigation right"@en ;
    skos:topConceptOf <http://www.neii.gov.au/def/voc/waterprogram/water-market-reports/Water-Market-Reports-glossary> ;
.

<http://www.neii.gov.au/def/voc/waterprogram/water-market-reports/permanent-trade>
    a skos:Concept ;
    dcterms:created "2020-09-07"^^xsd:date ;
    dcterms:creator <https://linked.data.gov.au/org/neii> ;
    skos:definition "Permanent trade has the same meaning as water access entitlement trade."@en ;
    skos:prefLabel "permanent trade"@en ;
    skos:relatedMatch <http://www.neii.gov.au/def/voc/waterprogram/water-market-reports/water-access-entitlement-trade> ;
    skos:topConceptOf <http://www.neii.gov.au/def/voc/waterprogram/water-market-reports/Water-Market-Reports-glossary> ;
.

<http://www.neii.gov.au/def/voc/waterprogram/water-market-reports/regulated-water-resource>
    a skos:Concept ;
    dcterms:created "2020-09-07"^^xsd:date ;
    dcterms:creator <https://linked.data.gov.au/org/neii> ;
    skos:definition "A water resource which has its flows controlled through the use of infrastructure to store and release water."@en ;
    skos:prefLabel "regulated water resource"@en ;
    skos:topConceptOf <http://www.neii.gov.au/def/voc/waterprogram/water-market-reports/Water-Market-Reports-glossary> ;
.

<http://www.neii.gov.au/def/voc/waterprogram/water-market-reports/reliability>
    a skos:Concept ;
    dcterms:created "2020-09-07"^^xsd:date ;
    dcterms:creator <https://linked.data.gov.au/org/neii> ;
    skos:definition """The frequency with which water allocated under a water access entitlement is able to be supplied in full.
Source: Intergovernmental Agreement on a National Water Initiative (http://www.bom.gov.au/water/about/consultation/document/NWI_2004.pdf) Schedule B(ii)"""@en ;
    skos:prefLabel "reliability"@en ;
    skos:topConceptOf <http://www.neii.gov.au/def/voc/waterprogram/water-market-reports/Water-Market-Reports-glossary> ;
.

<http://www.neii.gov.au/def/voc/waterprogram/water-market-reports/rural-water-utility>
    a skos:Concept ;
    dcterms:created "2020-09-07"^^xsd:date ;
    dcterms:creator <https://linked.data.gov.au/org/neii> ;
    skos:definition "An organisation that supplies water for irrigation, town and community use in a rural area."@en ;
    skos:prefLabel "rural water utility"@en ;
    skos:topConceptOf <http://www.neii.gov.au/def/voc/waterprogram/water-market-reports/Water-Market-Reports-glossary> ;
.

<http://www.neii.gov.au/def/voc/waterprogram/water-market-reports/stock-and-domestic-use>
    a skos:Concept ;
    dcterms:created "2020-09-07"^^xsd:date ;
    dcterms:creator <https://linked.data.gov.au/org/neii> ;
    skos:definition "Use of water for domestic consumption (e.g. drinking, cooking, washing, watering household gardens, filling swimming pools associated with domestic premises) and to water stock on a property. Does not include water used for irrigating crops that will be sold, bartered or used for stock fodder, for washing down machinery sheds, or for intensive livestock operations."@en ;
    skos:prefLabel "stock and domestic use"@en ;
    skos:topConceptOf <http://www.neii.gov.au/def/voc/waterprogram/water-market-reports/Water-Market-Reports-glossary> ;
.

<http://www.neii.gov.au/def/voc/waterprogram/water-market-reports/surface-water>
    a skos:Concept ;
    dcterms:created "2020-09-07"^^xsd:date ;
    dcterms:creator <https://linked.data.gov.au/org/neii> ;
    skos:definition """Includes: (a) water in a watercourse, lake or wetland and (b) any water flowing over or lying on land: (i) after having precipitated naturally or (ii) after having risen to the surface naturally from underground.
Source:  Water Act 2007 (https://www.legislation.gov.au/Details/C2018C00505) Part 1 Section 4, at 8 February 2019. For the latest information on Australian Government law please go to Federal Register of Legislation (https://www.legislation.gov.au/)"""@en ;
    skos:prefLabel "surface water"@en ;
    skos:topConceptOf <http://www.neii.gov.au/def/voc/waterprogram/water-market-reports/Water-Market-Reports-glossary> ;
.

<http://www.neii.gov.au/def/voc/waterprogram/water-market-reports/temporary-trade>
    a skos:Concept ;
    dcterms:created "2020-09-07"^^xsd:date ;
    dcterms:creator <https://linked.data.gov.au/org/neii> ;
    skos:definition "Temporary trade has the same meaning as water allocation trade."@en ;
    skos:prefLabel "temporary trade"@en ;
    skos:relatedMatch <http://www.neii.gov.au/def/voc/waterprogram/water-market-reports/water-allocation-trade> ;
    skos:topConceptOf <http://www.neii.gov.au/def/voc/waterprogram/water-market-reports/Water-Market-Reports-glossary> ;
.

<http://www.neii.gov.au/def/voc/waterprogram/water-market-reports/tradeable-water-rights>
    a skos:Concept ;
    dcterms:created "2020-09-07"^^xsd:date ;
    dcterms:creator <https://linked.data.gov.au/org/neii> ;
    skos:definition """Are: (a) water access rights, (b) water delivery rights or (c) irrigation rights.
Note: Some components within water access rights are not tradeable.
Source: Derived from the Water Act 2007 (https://www.legislation.gov.au/Details/C2018C00505) Part 1 Section 4, at 8 February 2019. For the latest information on Australian Government law please go to Federal Register of Legislation (https://www.legislation.gov.au/)"""@en ;
    skos:prefLabel "tradeable water rights"@en ;
    skos:topConceptOf <http://www.neii.gov.au/def/voc/waterprogram/water-market-reports/Water-Market-Reports-glossary> ;
.

<http://www.neii.gov.au/def/voc/waterprogram/water-market-reports/trading-zones>
    a skos:Concept ;
    dcterms:created "2020-09-07"^^xsd:date ;
    dcterms:creator <https://linked.data.gov.au/org/neii> ;
    skos:definition """Zones established to simplify administration of trade by setting out the known supply source or management arrangements and the physical realities of relevant supply systems within the zone.
Source: Derived from the Intergovernmental Agreement on a National Water Initiative (http://www.bom.gov.au/water/about/consultation/document/NWI_2004.pdf) Schedule B(i)"""@en ;
    skos:prefLabel "trading zones"@en ;
    skos:topConceptOf <http://www.neii.gov.au/def/voc/waterprogram/water-market-reports/Water-Market-Reports-glossary> ;
.

<http://www.neii.gov.au/def/voc/waterprogram/water-market-reports/transaction-costs>
    a skos:Concept ;
    dcterms:created "2020-09-07"^^xsd:date ;
    dcterms:creator <https://linked.data.gov.au/org/neii> ;
    skos:definition "Includes search, negotiation and enforcement costs including, but not limited to, all government water transfer fees and charges applicable to water trade, conveyance charges and professional service fees (such as accountants, brokers, lawyers)."@en ;
    skos:prefLabel "transaction costs"@en ;
    skos:topConceptOf <http://www.neii.gov.au/def/voc/waterprogram/water-market-reports/Water-Market-Reports-glossary> ;
.

<http://www.neii.gov.au/def/voc/waterprogram/water-market-reports/unbundled-right>
    a skos:Concept ;
    dcterms:created "2020-09-07"^^xsd:date ;
    dcterms:creator <https://linked.data.gov.au/org/neii> ;
    skos:definition """The separation of a bundled right into its individual elements. At its most basic level, unbundling separate water rights from a land property title, allowing the trade of the water rights independently of land.
Additional degrees of unbundling involve the separation of a water right into its individual elements. These might include, but are not limited to, water access entitlements, water allocations, water use rights, delivery rights and works approvals."""@en ;
    skos:prefLabel "unbundled right"@en ;
    skos:topConceptOf <http://www.neii.gov.au/def/voc/waterprogram/water-market-reports/Water-Market-Reports-glossary> ;
.

<http://www.neii.gov.au/def/voc/waterprogram/water-market-reports/unregulated-water-resource>
    a skos:Concept ;
    dcterms:created "2020-09-07"^^xsd:date ;
    dcterms:creator <https://linked.data.gov.au/org/neii> ;
    skos:definition "A water resource that is not controlled through the use of infrastructure to store and release water."@en ;
    skos:prefLabel "unregulated water resource"@en ;
    skos:topConceptOf <http://www.neii.gov.au/def/voc/waterprogram/water-market-reports/Water-Market-Reports-glossary> ;
.

<http://www.neii.gov.au/def/voc/waterprogram/water-market-reports/water-access-entitlement>
    a skos:Concept ;
    dcterms:created "2020-09-07"^^xsd:date ;
    dcterms:creator <https://linked.data.gov.au/org/neii> ;
    skos:definition """A perpetual or ongoing entitlement to exclusive access to a share of water from a specified consumptive pool as defined in the relevant water plan.
Source: Intergovernmental Agreement on a National Water Initiative (http://www.bom.gov.au/water/about/consultation/document/NWI_2004.pdf) Schedule B(ii)"""@en ;
    skos:prefLabel "water access entitlement"@en ;
    skos:topConceptOf <http://www.neii.gov.au/def/voc/waterprogram/water-market-reports/Water-Market-Reports-glossary> ;
.

<http://www.neii.gov.au/def/voc/waterprogram/water-market-reports/water-access-entitlement-type>
    a skos:Concept ;
    dcterms:created "2020-09-07"^^xsd:date ;
    dcterms:creator <https://linked.data.gov.au/org/neii> ;
    skos:definition "Water right types as defined in State and Territory legislation which includes bundled and unbundled water rights and bulk water access entitlements."@en ;
    skos:prefLabel "water access entitlement type"@en ;
    skos:topConceptOf <http://www.neii.gov.au/def/voc/waterprogram/water-market-reports/Water-Market-Reports-glossary> ;
.

<http://www.neii.gov.au/def/voc/waterprogram/water-market-reports/water-access-entitlement-volume>
    a skos:Concept ;
    dcterms:created "2020-09-07"^^xsd:date ;
    dcterms:creator <https://linked.data.gov.au/org/neii> ;
    skos:definition "The share, nominal volume or extraction rate associated with a water access entitlement."@en ;
    skos:prefLabel "water access entitlement volume"@en ;
    skos:topConceptOf <http://www.neii.gov.au/def/voc/waterprogram/water-market-reports/Water-Market-Reports-glossary> ;
.

<http://www.neii.gov.au/def/voc/waterprogram/water-market-reports/water-access-entitlements-on-issue>
    a skos:Concept ;
    dcterms:created "2020-09-07"^^xsd:date ;
    dcterms:creator <https://linked.data.gov.au/org/neii> ;
    skos:definition "The total quantity of water access entitlements granted by State and Territory government water agencies which are in effect at a given point in time."@en ;
    skos:prefLabel "water access entitlements on issue"@en ;
    skos:topConceptOf <http://www.neii.gov.au/def/voc/waterprogram/water-market-reports/Water-Market-Reports-glossary> ;
.

<http://www.neii.gov.au/def/voc/waterprogram/water-market-reports/water-access-right>
    a skos:Concept ;
    dcterms:created "2020-09-07"^^xsd:date ;
    dcterms:creator <https://linked.data.gov.au/org/neii> ;
    skos:definition """Water access right: (a) any right conferred by or under a law of a State to do either or both of the following: (i) to hold water from a water resource or (ii) to take water from a water resource and (b) without limiting paragraph (a) includes the following rights of the kind referred to in that paragraph: (i) stock and domestic rights, (ii) riparian rights, (iii) a water access entitlement or (iv) a water allocation and (c) includes any other right in relation to the taking or use of water that is prescribed by the regulations for the purposes of this paragraph.
Source:  Water Act 2007 (https://www.legislation.gov.au/Details/C2018C00505) Part 1 Section 4, at 8 February 2019. For the latest information on Australian Government law please go to Federal Register of Legislation (https://www.legislation.gov.au/)"""@en ;
    skos:prefLabel "water access right"@en ;
    skos:topConceptOf <http://www.neii.gov.au/def/voc/waterprogram/water-market-reports/Water-Market-Reports-glossary> ;
.

<http://www.neii.gov.au/def/voc/waterprogram/water-market-reports/water-delivery-right>
    a skos:Concept ;
    dcterms:created "2020-09-07"^^xsd:date ;
    dcterms:creator <https://linked.data.gov.au/org/neii> ;
    skos:definition """A right to have water delivered by an infrastructure operator.
Source:  Water Act 2007 (https://www.legislation.gov.au/Details/C2018C00505) Part 1 Section 4, at 8 February 2019. For the latest information on Australian Government law please go to Federal Register of Legislation (https://www.legislation.gov.au/)"""@en ;
    skos:prefLabel "water delivery right"@en ;
    skos:topConceptOf <http://www.neii.gov.au/def/voc/waterprogram/water-market-reports/Water-Market-Reports-glossary> ;
.

<http://www.neii.gov.au/def/voc/waterprogram/water-market-reports/water-lease>
    a skos:Concept ;
    dcterms:created "2020-09-07"^^xsd:date ;
    dcterms:creator <https://linked.data.gov.au/org/neii> ;
    skos:definition "A transaction to transfer a water right from one legal entity to another, in whole or in part, for a specified period of time which involves an exchange of a monetary value."@en ;
    skos:prefLabel "water lease"@en ;
    skos:topConceptOf <http://www.neii.gov.au/def/voc/waterprogram/water-market-reports/Water-Market-Reports-glossary> ;
.

<http://www.neii.gov.au/def/voc/waterprogram/water-market-reports/water-market-equivalent-terms>
    a skos:Concept ;
    dcterms:created "2020-09-07"^^xsd:date ;
    dcterms:creator <https://linked.data.gov.au/org/neii> ;
    skos:definition "Equivalent National, State and Territory water market product and trading terms"@en ;
    skos:prefLabel "water market equivalent terms"@en ;
    skos:topConceptOf <http://www.neii.gov.au/def/voc/waterprogram/water-market-reports/Water-Market-Reports-glossary> ;
.

<http://www.neii.gov.au/def/voc/waterprogram/water-market-reports/water-plan>
    a skos:Concept ;
    dcterms:created "2020-09-07"^^xsd:date ;
    dcterms:creator <https://linked.data.gov.au/org/neii> ;
    skos:definition "Statutory plans for surface and/or groundwater systems, consistent with the Regional Natural Resource Management Plans, developed in consultation with all relevant stakeholders on the basis of best scientific and socio-economic assessment, to provide secure ecological outcomes and resource security for users."@en ;
    skos:prefLabel "water plan"@en ;
    skos:topConceptOf <http://www.neii.gov.au/def/voc/waterprogram/water-market-reports/Water-Market-Reports-glossary> ;
.

<http://www.neii.gov.au/def/voc/waterprogram/water-market-reports/water-provider>
    a skos:Concept ;
    dcterms:created "2020-09-07"^^xsd:date ;
    dcterms:creator <https://linked.data.gov.au/org/neii> ;
    skos:definition """A business or organisation that provides a reticulated water supply, irrigation water, reused or recycled water, or a bulk water supply service. Water providers may be Government or private and often operate water storage, purification and supply services. They may also provide sewerage or drainage services.
Source: © Commonwealth of Australia 2005, National Water Commission, Australian Water Resources 2005, Glossary and definitions."""@en ;
    skos:prefLabel "water provider"@en ;
    skos:topConceptOf <http://www.neii.gov.au/def/voc/waterprogram/water-market-reports/Water-Market-Reports-glossary> ;
.

<http://www.neii.gov.au/def/voc/waterprogram/water-market-reports/water-resource>
    a skos:Concept ;
    dcterms:created "2020-09-07"^^xsd:date ;
    dcterms:creator <https://linked.data.gov.au/org/neii> ;
    skos:definition """Means: (a) surface water or groundwater, or (b) a watercourse, lake, wetland or aquifer (whether or not it currently has water in it), and includes all aspects of the water resource (including water, organisms and other components and ecosystems that contribute to the physical state and environmental value of the water resource).
Source:  Water Act 2007 (https://www.legislation.gov.au/Details/C2018C00505) Part 1 Section 4, at 8 February 2019. For the latest information on Australian Government law please go to Federal Register of Legislation (https://www.legislation.gov.au/)"""@en ;
    skos:prefLabel "water resource"@en ;
    skos:topConceptOf <http://www.neii.gov.au/def/voc/waterprogram/water-market-reports/Water-Market-Reports-glossary> ;
.

<http://www.neii.gov.au/def/voc/waterprogram/water-market-reports/water-resource-plan>
    a skos:Concept ;
    dcterms:created "2020-09-07"^^xsd:date ;
    dcterms:creator <https://linked.data.gov.au/org/neii> ;
    skos:definition "A plan for the management of a water resource."@en ;
    skos:prefLabel "water resource plan"@en ;
    skos:topConceptOf <http://www.neii.gov.au/def/voc/waterprogram/water-market-reports/Water-Market-Reports-glossary> ;
.

<http://www.neii.gov.au/def/voc/waterprogram/water-market-reports/water-resource-plan-area>
    a skos:Concept ;
    dcterms:created "2020-09-07"^^xsd:date ;
    dcterms:creator <https://linked.data.gov.au/org/neii> ;
    skos:definition "Water resource area defined in a water resource plan."@en ;
    skos:prefLabel "water resource plan area"@en ;
    skos:topConceptOf <http://www.neii.gov.au/def/voc/waterprogram/water-market-reports/Water-Market-Reports-glossary> ;
.

<http://www.neii.gov.au/def/voc/waterprogram/water-market-reports/water-resource-type>
    a skos:Concept ;
    dcterms:created "2020-09-07"^^xsd:date ;
    dcterms:creator <https://linked.data.gov.au/org/neii> ;
    skos:definition "Describes the attributes of a water resource, e.g. surface or groundwater, regulated or unregulated water."@en ;
    skos:prefLabel "water resource type"@en ;
    skos:topConceptOf <http://www.neii.gov.au/def/voc/waterprogram/water-market-reports/Water-Market-Reports-glossary> ;
.

<http://www.neii.gov.au/def/voc/waterprogram/water-market-reports/water-right>
    a skos:Concept ;
    dcterms:created "2020-09-07"^^xsd:date ;
    dcterms:creator <https://linked.data.gov.au/org/neii> ;
    skos:definition "A generic term for the range of different tradeable and non-tradeable water rights across Australia. These might include, but are not limited to, water access entitlements, water allocations, water use rights, delivery rights, irrigation rights and works approvals."@en ;
    skos:prefLabel "water right"@en ;
    skos:topConceptOf <http://www.neii.gov.au/def/voc/waterprogram/water-market-reports/Water-Market-Reports-glossary> ;
.

<http://www.neii.gov.au/def/voc/waterprogram/water-market-reports/water-tagging>
    a skos:Concept ;
    dcterms:created "2020-09-07"^^xsd:date ;
    dcterms:creator <https://linked.data.gov.au/org/neii> ;
    skos:definition """An accounting approach that allows a traded water access entitlement to retain its original characteristics when traded to a new jurisdiction and/or trading zone, rather than being converted into a form issued in the new jurisdiction and/or trading zone.
Source: Intergovernmental Agreement on a National Water Initiative (http://www.bom.gov.au/water/about/consultation/document/NWI_2004.pdf) Schedule B(i)"""@en ;
    skos:prefLabel "water tagging"@en ;
    skos:topConceptOf <http://www.neii.gov.au/def/voc/waterprogram/water-market-reports/Water-Market-Reports-glossary> ;
.

<http://www.neii.gov.au/def/voc/waterprogram/water-market-reports/water-trade>
    a skos:Concept ;
    dcterms:created "2020-09-07"^^xsd:date ;
    dcterms:creator <https://linked.data.gov.au/org/neii> ;
    skos:definition "A transaction to buy, sell or lease a water right, in whole or in part, from one legal entity to another."@en ;
    skos:prefLabel "water trade"@en ;
    skos:topConceptOf <http://www.neii.gov.au/def/voc/waterprogram/water-market-reports/Water-Market-Reports-glossary> ;
.

<http://www.neii.gov.au/def/voc/waterprogram/water-market-reports/water-trade-price>
    a skos:Concept ;
    dcterms:created "2020-09-07"^^xsd:date ;
    dcterms:creator <https://linked.data.gov.au/org/neii> ;
    skos:definition "Water price or trade price has the same meaning as net water price"@en ;
    skos:prefLabel "water trade price"@en ;
    skos:relatedMatch <http://www.neii.gov.au/def/voc/waterprogram/water-market-reports/net-water-price> ;
    skos:topConceptOf <http://www.neii.gov.au/def/voc/waterprogram/water-market-reports/Water-Market-Reports-glossary> ;
.

<http://www.neii.gov.au/def/voc/waterprogram/water-market-reports/water-year>
    a skos:Concept ;
    dcterms:created "2020-09-07"^^xsd:date ;
    dcterms:creator <https://linked.data.gov.au/org/neii> ;
    skos:definition "1 July to 30 June"@en ;
    skos:prefLabel "water year"@en ;
    skos:topConceptOf <http://www.neii.gov.au/def/voc/waterprogram/water-market-reports/Water-Market-Reports-glossary> ;
.

<http://editor.vocabs.ands.org.au/user/312e891c-ecf1-44e3-a666-e0e6efb60a18>
    a dcterms:Agent ;
    foaf:name "Water Program, Bureau of Meteorology" ;
.

<http://www.neii.gov.au/def/voc/waterprogram/water-market-reports/IIO>
    a skos:Concept ;
    dcterms:created "2020-09-07"^^xsd:date ;
    dcterms:creator <https://linked.data.gov.au/org/neii> ;
    skos:definition """irrigation infrastructure operator
An entity that operates water service infrastructure for the purposes of delivering water for the primary purpose of it being used for irrigation.
Source: Water Act 2007 (https://www.legislation.gov.au/Details/C2018C00505) Part 1 Section 7, at 8 February 2019. For the latest information on Australian Government law please go to Federal Register of Legislation (https://www.legislation.gov.au/)"""@en ;
    skos:prefLabel "IIO"@en ;
    skos:relatedMatch <http://www.neii.gov.au/def/voc/waterprogram/water-market-reports/irrigation-infrastructure-operator> ;
    skos:topConceptOf <http://www.neii.gov.au/def/voc/waterprogram/water-market-reports/Water-Market-Reports-glossary> ;
.

<http://www.neii.gov.au/def/voc/waterprogram/water-market-reports/NWI>
    a skos:Concept ;
    dcterms:created "2020-09-07"^^xsd:date ;
    dcterms:creator <https://linked.data.gov.au/org/neii> ;
    skos:definition "National Water Initiative"@en ;
    skos:prefLabel "NWI"@en ;
    skos:relatedMatch <http://www.neii.gov.au/def/voc/waterprogram/water-market-reports/National-Water-Initiative> ;
    skos:topConceptOf <http://www.neii.gov.au/def/voc/waterprogram/water-market-reports/Water-Market-Reports-glossary> ;
.

<http://www.neii.gov.au/def/voc/waterprogram/water-market-reports/National-Water-Initiative>
    a skos:Concept ;
    dcterms:created "2020-09-07"^^xsd:date ;
    dcterms:creator <https://linked.data.gov.au/org/neii> ;
    skos:definition """The Intergovernmental Agreement on a National Water Initiative between the Commonwealth of Australia and the Governments of New South Wales, Victoria, Queensland, South Australia, Western Australia, Tasmania, the Australian Capital Territory and the Northern Territory (as amended from time to time).
Source: Water Act 2007 (https://www.legislation.gov.au/Details/C2018C00505) Part 1 Section 4, at 8 February 2019. For the latest information on Australian Government law please go to Federal Register of Legislation (https://www.legislation.gov.au/)"""@en ;
    skos:prefLabel "National Water Initiative"@en ;
    skos:relatedMatch <http://www.neii.gov.au/def/voc/waterprogram/water-market-reports/NWI> ;
    skos:topConceptOf <http://www.neii.gov.au/def/voc/waterprogram/water-market-reports/Water-Market-Reports-glossary> ;
.

<http://www.neii.gov.au/def/voc/waterprogram/water-market-reports/VWAP>
    a skos:Concept ;
    dcterms:created "2020-09-07"^^xsd:date ;
    dcterms:creator <https://linked.data.gov.au/org/neii> ;
    skos:definition """volume weighted average price
The average value (dollars per megalitre) of the water traded where each trade is weighted proportionally by the volume of water (in megalitre) involved in the sale. This provides a more accurate representation of the price (i.e. high volume trades generally attract a ‘bulk discount’)."""@en ;
    skos:prefLabel "VWAP"@en ;
    skos:relatedMatch <http://www.neii.gov.au/def/voc/waterprogram/water-market-reports/volume-weighted-average-price> ;
    skos:topConceptOf <http://www.neii.gov.au/def/voc/waterprogram/water-market-reports/Water-Market-Reports-glossary> ;
.

<http://www.neii.gov.au/def/voc/waterprogram/water-market-reports/allocation>
    a skos:Concept ;
    dcterms:created "2020-09-07"^^xsd:date ;
    dcterms:creator <https://linked.data.gov.au/org/neii> ;
    skos:definition "The specific volume of water allocated to water access entitlements in a given water year or allocated as specified within a water resource plan."@en ;
    skos:prefLabel "allocation"@en ;
    skos:relatedMatch <http://www.neii.gov.au/def/voc/waterprogram/water-market-reports/water-allocation> ;
    skos:topConceptOf <http://www.neii.gov.au/def/voc/waterprogram/water-market-reports/Water-Market-Reports-glossary> ;
.

<http://www.neii.gov.au/def/voc/waterprogram/water-market-reports/groundwater-system>
    a skos:Concept ;
    dcterms:created "2020-09-07"^^xsd:date ;
    dcterms:creator <https://linked.data.gov.au/org/neii> ;
    skos:definition "A collective term for areas that are defined normally at a higher level than groundwater management area, for the purposes of water data reporting."@en ;
    skos:prefLabel "groundwater system"@en ;
    skos:relatedMatch <http://www.neii.gov.au/def/voc/waterprogram/water-market-reports/water-system> ;
    skos:topConceptOf <http://www.neii.gov.au/def/voc/waterprogram/water-market-reports/Water-Market-Reports-glossary> ;
.

<http://www.neii.gov.au/def/voc/waterprogram/water-market-reports/irrigation-infrastructure-operator>
    a skos:Concept ;
    dcterms:created "2020-09-07"^^xsd:date ;
    dcterms:creator <https://linked.data.gov.au/org/neii> ;
    skos:definition """An entity that operates water service infrastructure for the purposes of delivering water for the primary purpose of it being used for irrigation.
Source: Adapted from the Water Act 2007 (https://www.legislation.gov.au/Details/C2018C00505) Part 1 Section 7, at 8 February 2019. For the latest information on Australian Government law please go to Federal Register of Legislation (https://www.legislation.gov.au/)"""@en ;
    skos:prefLabel "irrigation infrastructure operator"@en ;
    skos:relatedMatch <http://www.neii.gov.au/def/voc/waterprogram/water-market-reports/IIO> ;
    skos:topConceptOf <http://www.neii.gov.au/def/voc/waterprogram/water-market-reports/Water-Market-Reports-glossary> ;
.

<http://www.neii.gov.au/def/voc/waterprogram/water-market-reports/net-water-price>
    a skos:Concept ;
    dcterms:created "2020-09-07"^^xsd:date ;
    dcterms:creator <https://linked.data.gov.au/org/neii> ;
    skos:definition "The transfer price of water as agreed between legal entities exclusive of all applicable transaction costs."@en ;
    skos:prefLabel "net water price"@en ;
    skos:topConceptOf <http://www.neii.gov.au/def/voc/waterprogram/water-market-reports/Water-Market-Reports-glossary> ;
.

<http://www.neii.gov.au/def/voc/waterprogram/water-market-reports/planned-environmental-water>
    a skos:Concept ;
    dcterms:created "2020-09-07"^^xsd:date ;
    dcterms:creator <https://linked.data.gov.au/org/neii> ;
    skos:definition "Planned environmental water is committed in a water plan for achieving environmental outcomes."@en ;
    skos:prefLabel "planned environmental water"@en ;
    skos:topConceptOf <http://www.neii.gov.au/def/voc/waterprogram/water-market-reports/Water-Market-Reports-glossary> ;
.

<http://www.neii.gov.au/def/voc/waterprogram/water-market-reports/product>
    a skos:Concept ;
    dcterms:created "2020-09-07"^^xsd:date ;
    dcterms:creator <https://linked.data.gov.au/org/neii> ;
    skos:definition "A water right that is tradeable, falling under the broad category of either water access entitlement or water allocation. A product may be bundled or unbundled and has various attributes such as water resource type (e.g. surface water, groundwater, regulated, unregulated) and reliability type (e.g. high, low priority)."@en ;
    skos:prefLabel "product"@en ;
    skos:relatedMatch <http://www.neii.gov.au/def/voc/waterprogram/water-market-reports/water-product> ;
    skos:topConceptOf <http://www.neii.gov.au/def/voc/waterprogram/water-market-reports/Water-Market-Reports-glossary> ;
.

<http://www.neii.gov.au/def/voc/waterprogram/water-market-reports/surface-water-system>
    a skos:Concept ;
    dcterms:created "2020-09-07"^^xsd:date ;
    dcterms:creator <https://linked.data.gov.au/org/neii> ;
    skos:definition "An area that is hydrologically connected and defined, normally at a higher level than surface water management area, for the purposes of water data reporting."@en ;
    skos:prefLabel "surface water system"@en ;
    skos:relatedMatch <http://www.neii.gov.au/def/voc/waterprogram/water-market-reports/water-system> ;
    skos:topConceptOf <http://www.neii.gov.au/def/voc/waterprogram/water-market-reports/Water-Market-Reports-glossary> ;
.

<http://www.neii.gov.au/def/voc/waterprogram/water-market-reports/volume-weighted-average-price>
    a skos:Concept ;
    dcterms:created "2020-09-07"^^xsd:date ;
    dcterms:creator <https://linked.data.gov.au/org/neii> ;
    skos:definition "The average value (dollars per megalitre) of  the water traded where each trade is weighted proportionally by the volume of water (in megalitre) involved in the sale. This provides a more accurate representation of the price (i.e. high volume trades generally attract a ‘bulk discount’)."@en ;
    skos:prefLabel "volume weighted average price"@en ;
    skos:relatedMatch <http://www.neii.gov.au/def/voc/waterprogram/water-market-reports/VWAP> ;
    skos:topConceptOf <http://www.neii.gov.au/def/voc/waterprogram/water-market-reports/Water-Market-Reports-glossary> ;
.

<http://www.neii.gov.au/def/voc/waterprogram/water-market-reports/water-access-entitlement-trade>
    a skos:Concept ;
    dcterms:created "2020-09-07"^^xsd:date ;
    dcterms:creator <https://linked.data.gov.au/org/neii> ;
    skos:definition "A transaction to transfer a water access entitlement from one legal entity to another, with or without a change in location, perpetually or for a specified term (i.e. lease)."@en ;
    skos:prefLabel "water access entitlement trade"@en ;
    skos:topConceptOf <http://www.neii.gov.au/def/voc/waterprogram/water-market-reports/Water-Market-Reports-glossary> ;
.

<http://www.neii.gov.au/def/voc/waterprogram/water-market-reports/water-allocation>
    a skos:Concept ;
    dcterms:created "2020-09-07"^^xsd:date ;
    dcterms:creator <https://linked.data.gov.au/org/neii> ;
    skos:definition """The specific volume of water allocated to water access entitlements in a given water year or allocated as specified within a water resource plan.
Source:  Water Act 2007 (https://www.legislation.gov.au/Details/C2018C00505) Part 1 Section 4, at 8 February 2019. For the latest information on Australian Government law please go to Federal Register of Legislation (https://www.legislation.gov.au/)"""@en ;
    skos:prefLabel "water allocation"@en ;
    skos:relatedMatch <http://www.neii.gov.au/def/voc/waterprogram/water-market-reports/allocation> ;
    skos:topConceptOf <http://www.neii.gov.au/def/voc/waterprogram/water-market-reports/Water-Market-Reports-glossary> ;
.

<http://www.neii.gov.au/def/voc/waterprogram/water-market-reports/water-allocation-trade>
    a skos:Concept ;
    dcterms:created "2020-09-07"^^xsd:date ;
    dcterms:creator <https://linked.data.gov.au/org/neii> ;
    skos:definition """A transaction to transfer a water allocation from one legal entity to another, with or without a change in location, for the remaining water year (by default) or for a specified term that may be less than the end of the water year or carried over to subsequent years (i.e. lease).
Water allocation trade is used in preference to temporary trade in the National Water Initiative."""@en ;
    skos:prefLabel "water allocation trade"@en ;
    skos:relatedMatch <http://www.neii.gov.au/def/voc/waterprogram/water-market-reports/planned-environmental-water> ;
    skos:topConceptOf <http://www.neii.gov.au/def/voc/waterprogram/water-market-reports/Water-Market-Reports-glossary> ;
.

<http://www.neii.gov.au/def/voc/waterprogram/water-market-reports/water-product>
    a skos:Concept ;
    dcterms:created "2020-09-07"^^xsd:date ;
    dcterms:creator <https://linked.data.gov.au/org/neii> ;
    skos:definition "A water right that is tradeable, falling under the broad category of either water access entitlement or water allocation. A product may be bundled or unbundled and has various attributes such as water resource type (e.g. surface water, groundwater, regulated, unregulated) and reliability type (e.g. high, low priority)."@en ;
    skos:prefLabel "water product"@en ;
    skos:relatedMatch <http://www.neii.gov.au/def/voc/waterprogram/water-market-reports/product> ;
    skos:topConceptOf <http://www.neii.gov.au/def/voc/waterprogram/water-market-reports/Water-Market-Reports-glossary> ;
.

<http://www.neii.gov.au/def/voc/waterprogram/water-market-reports/water-system>
    a skos:Concept ;
    dcterms:created "2020-09-07"^^xsd:date ;
    dcterms:creator <https://linked.data.gov.au/org/neii> ;
    skos:definition """A system that is hydrologically connected and defined, normally at a higher level than surface or groundwater management area, for the purpose of water data reporting (e.g. sub-catchment, catchment, basin or drainage division and/or groundwater management unit, sub-aquifer, aquifer, groundwater basin).
Source: Intergovernmental Agreement on a National Water Initiative (http://www.bom.gov.au/water/about/consultation/document/NWI_2004.pdf) Schedule B(i)"""@en ;
    skos:prefLabel "water system"@en ;
    skos:relatedMatch
        <http://www.neii.gov.au/def/voc/waterprogram/water-market-reports/groundwater-system> ,
        <http://www.neii.gov.au/def/voc/waterprogram/water-market-reports/surface-water-system> ;
    skos:topConceptOf <http://www.neii.gov.au/def/voc/waterprogram/water-market-reports/Water-Market-Reports-glossary> ;
.

<http://www.neii.gov.au/def/voc/waterprogram/water-market-reports/Water-Market-Reports-glossary>
    a skos:ConceptScheme ;
    dcterms:contributor <http://editor.vocabs.ands.org.au/user/312e891c-ecf1-44e3-a666-e0e6efb60a18> ;
    dcterms:created "2020-09-07"^^xsd:date ;
    dcterms:creator <https://linked.data.gov.au/org/neii> ;
    dcterms:description "This glossary provides definitions of terms and acronyms used in the Bureau of Meteorology's water markets dashboard."@en ;
    dcterms:issued "2020-09-07" ;
    dcterms:publisher <http://editor.vocabs.ands.org.au/user/312e891c-ecf1-44e3-a666-e0e6efb60a18> ;
    dcterms:subject "Water Market Reports glossary"@en ;
    dcterms:title "Water Market Reports glossary"@en ;
    owl:versionInfo "Version 1" ;
    skos:hasTopConcept
        <http://www.neii.gov.au/def/voc/waterprogram/water-market-reports/IIO> ,
        <http://www.neii.gov.au/def/voc/waterprogram/water-market-reports/NWI> ,
        <http://www.neii.gov.au/def/voc/waterprogram/water-market-reports/National-Water-Initiative> ,
        <http://www.neii.gov.au/def/voc/waterprogram/water-market-reports/Non-consumptive-use> ,
        <http://www.neii.gov.au/def/voc/waterprogram/water-market-reports/VWAP> ,
        <http://www.neii.gov.au/def/voc/waterprogram/water-market-reports/allocation> ,
        <http://www.neii.gov.au/def/voc/waterprogram/water-market-reports/allocation-volume> ,
        <http://www.neii.gov.au/def/voc/waterprogram/water-market-reports/available-water> ,
        <http://www.neii.gov.au/def/voc/waterprogram/water-market-reports/bulk-water> ,
        <http://www.neii.gov.au/def/voc/waterprogram/water-market-reports/bulk-water-access-entitlement> ,
        <http://www.neii.gov.au/def/voc/waterprogram/water-market-reports/bundled-right> ,
        <http://www.neii.gov.au/def/voc/waterprogram/water-market-reports/carryover> ,
        <http://www.neii.gov.au/def/voc/waterprogram/water-market-reports/catchment-area> ,
        <http://www.neii.gov.au/def/voc/waterprogram/water-market-reports/consumptive-pool> ,
        <http://www.neii.gov.au/def/voc/waterprogram/water-market-reports/consumptive-use> ,
        <http://www.neii.gov.au/def/voc/waterprogram/water-market-reports/external-trade> ,
        <http://www.neii.gov.au/def/voc/waterprogram/water-market-reports/gross-water-price> ,
        <http://www.neii.gov.au/def/voc/waterprogram/water-market-reports/groundwater> ,
        <http://www.neii.gov.au/def/voc/waterprogram/water-market-reports/groundwater-system> ,
        <http://www.neii.gov.au/def/voc/waterprogram/water-market-reports/held-environmental-water> ,
        <http://www.neii.gov.au/def/voc/waterprogram/water-market-reports/inflows> ,
        <http://www.neii.gov.au/def/voc/waterprogram/water-market-reports/internal-trade> ,
        <http://www.neii.gov.au/def/voc/waterprogram/water-market-reports/interstate-trade> ,
        <http://www.neii.gov.au/def/voc/waterprogram/water-market-reports/intrastate-trade> ,
        <http://www.neii.gov.au/def/voc/waterprogram/water-market-reports/irrigation-infrastructure-operator> ,
        <http://www.neii.gov.au/def/voc/waterprogram/water-market-reports/irrigation-right> ,
        <http://www.neii.gov.au/def/voc/waterprogram/water-market-reports/net-water-price> ,
        <http://www.neii.gov.au/def/voc/waterprogram/water-market-reports/permanent-trade> ,
        <http://www.neii.gov.au/def/voc/waterprogram/water-market-reports/planned-environmental-water> ,
        <http://www.neii.gov.au/def/voc/waterprogram/water-market-reports/product> ,
        <http://www.neii.gov.au/def/voc/waterprogram/water-market-reports/regulated-water-resource> ,
        <http://www.neii.gov.au/def/voc/waterprogram/water-market-reports/reliability> ,
        <http://www.neii.gov.au/def/voc/waterprogram/water-market-reports/rural-water-utility> ,
        <http://www.neii.gov.au/def/voc/waterprogram/water-market-reports/stock-and-domestic-use> ,
        <http://www.neii.gov.au/def/voc/waterprogram/water-market-reports/surface-water> ,
        <http://www.neii.gov.au/def/voc/waterprogram/water-market-reports/surface-water-system> ,
        <http://www.neii.gov.au/def/voc/waterprogram/water-market-reports/temporary-trade> ,
        <http://www.neii.gov.au/def/voc/waterprogram/water-market-reports/tradeable-water-rights> ,
        <http://www.neii.gov.au/def/voc/waterprogram/water-market-reports/trading-zones> ,
        <http://www.neii.gov.au/def/voc/waterprogram/water-market-reports/transaction-costs> ,
        <http://www.neii.gov.au/def/voc/waterprogram/water-market-reports/unbundled-right> ,
        <http://www.neii.gov.au/def/voc/waterprogram/water-market-reports/unregulated-water-resource> ,
        <http://www.neii.gov.au/def/voc/waterprogram/water-market-reports/volume-weighted-average-price> ,
        <http://www.neii.gov.au/def/voc/waterprogram/water-market-reports/water-access-entitlement> ,
        <http://www.neii.gov.au/def/voc/waterprogram/water-market-reports/water-access-entitlement-trade> ,
        <http://www.neii.gov.au/def/voc/waterprogram/water-market-reports/water-access-entitlement-type> ,
        <http://www.neii.gov.au/def/voc/waterprogram/water-market-reports/water-access-entitlement-volume> ,
        <http://www.neii.gov.au/def/voc/waterprogram/water-market-reports/water-access-entitlements-on-issue> ,
        <http://www.neii.gov.au/def/voc/waterprogram/water-market-reports/water-access-right> ,
        <http://www.neii.gov.au/def/voc/waterprogram/water-market-reports/water-allocation> ,
        <http://www.neii.gov.au/def/voc/waterprogram/water-market-reports/water-allocation-trade> ,
        <http://www.neii.gov.au/def/voc/waterprogram/water-market-reports/water-delivery-right> ,
        <http://www.neii.gov.au/def/voc/waterprogram/water-market-reports/water-lease> ,
        <http://www.neii.gov.au/def/voc/waterprogram/water-market-reports/water-market-equivalent-terms> ,
        <http://www.neii.gov.au/def/voc/waterprogram/water-market-reports/water-plan> ,
        <http://www.neii.gov.au/def/voc/waterprogram/water-market-reports/water-product> ,
        <http://www.neii.gov.au/def/voc/waterprogram/water-market-reports/water-provider> ,
        <http://www.neii.gov.au/def/voc/waterprogram/water-market-reports/water-resource> ,
        <http://www.neii.gov.au/def/voc/waterprogram/water-market-reports/water-resource-plan> ,
        <http://www.neii.gov.au/def/voc/waterprogram/water-market-reports/water-resource-plan-area> ,
        <http://www.neii.gov.au/def/voc/waterprogram/water-market-reports/water-resource-type> ,
        <http://www.neii.gov.au/def/voc/waterprogram/water-market-reports/water-right> ,
        <http://www.neii.gov.au/def/voc/waterprogram/water-market-reports/water-system> ,
        <http://www.neii.gov.au/def/voc/waterprogram/water-market-reports/water-tagging> ,
        <http://www.neii.gov.au/def/voc/waterprogram/water-market-reports/water-trade> ,
        <http://www.neii.gov.au/def/voc/waterprogram/water-market-reports/water-trade-price> ,
        <http://www.neii.gov.au/def/voc/waterprogram/water-market-reports/water-year> ;
.

<https://linked.data.gov.au/org/neii>
    a
        dcterms:Agent ,
        schema:Organization ;
    foaf:homepage "http://www.bom.gov.au/environment/transition.shtml"^^xsd:anyURI ;
    foaf:name "NEII" ;
.
